Bdd/Evaluate.lean
@@ -20,7 +20,7 @@ lemma evaluate_evaluate : evaluate O = OBdd.evaluate O := by
   next j hj =>
     have := evaluate_evaluate (O := O.low hj)
     have := evaluate_evaluate (O := O.high hj)
-    simp [OBdd.evaluate_node'' hj, *]
+    simp only [Pointer.node.injEq, OBdd.evaluate_node, *]
 termination_by O
 
 lemma evaluate_terminal {O : OBdd n m} : O.1.root = .terminal b → evaluate O = Function.const _ b := by
@@ -30,7 +30,7 @@ lemma evaluate_terminal {O : OBdd n m} : O.1.root = .terminal b → evaluate O =
 lemma evaluate_node {O : OBdd n m} (h : O.1.root = .node j) :
     evaluate O = fun I ↦ if I[O.1.heap[j].var] then evaluate (O.high h) I else evaluate (O.low h) I := by
   rw [evaluate_evaluate]
-  rw [OBdd.evaluate_node'' h]
+  rw [OBdd.evaluate_node' h]
   simp [evaluate_evaluate]
 
 /--
